Term_algebra.v
@@ -3,102 +3,102 @@ Require Import Env.
 
 Module Type Algebra.
 
-Variable signature: domain_env -> Type.
+Local Parameter signature: domain_env -> Type.
 
-Variables term args occ_term occ_args : Set.
+Local Parameters term args occ_term occ_args : Set.
 
-Variable mkVar : positive -> term.
+Local Parameter mkVar : positive -> term.
 
-Variable term_eq : term -> term -> bool.
-Variable args_eq : args -> args -> bool.
+Local Parameter term_eq : term -> term -> bool.
+Local Parameter args_eq : args -> args -> bool.
 
-Variable refl_term_eq : forall t:term,term_eq t t=true.
-Variable refl_args_eq : forall a:args,args_eq a a=true.
+Local Parameter refl_term_eq : forall t:term,term_eq t t=true.
+Local Parameter refl_args_eq : forall a:args,args_eq a a=true.
 
-Variable inst_term : term -> nat -> term -> term.
-Variable inst_args : term -> nat -> args -> args.
+Local Parameter inst_term : term -> nat -> term -> term.
+Local Parameter inst_args : term -> nat -> args -> args.
 
-Variable rewrite_term : term -> term -> occ_term -> term -> option term.
-Variable rewrite_args : term -> term -> occ_args -> args -> option args.
+Local Parameter rewrite_term : term -> term -> occ_term -> term -> option term.
+Local Parameter rewrite_args : term -> term -> occ_args -> args -> option args.
 
-Variable check_ground_term : 
+Local Parameter check_ground_term : 
    forall Denv, signature Denv -> var_ctx -> term -> domain -> bool.
-Variable WF_ground_term : 
+Local Parameter WF_ground_term : 
    forall Denv, signature Denv -> var_ctx -> term -> domain -> Prop.
-Variable WF_checked_ground_term :
+Local Parameter WF_checked_ground_term :
   forall Denv Sigma vars t dom, 
   check_ground_term Denv Sigma vars t dom = true ->
   WF_ground_term Denv Sigma vars t dom.
 
-Variable check_term : forall Denv,
+Local Parameter check_term : forall Denv,
   signature Denv -> var_ctx -> rel_ctx -> term -> domain -> bool.
-Variable check_args : forall Denv,
+Local Parameter check_args : forall Denv,
   signature Denv -> var_ctx -> rel_ctx -> args -> arity -> bool.
 
-Variable WF_term : forall Denv,
+Local Parameter WF_term : forall Denv,
   signature Denv -> var_ctx -> rel_ctx -> term -> domain -> Prop.
-Variable WF_args : forall Denv,
+Local Parameter WF_args : forall Denv,
   signature Denv -> var_ctx -> rel_ctx -> args -> arity -> Prop.
 
-Variable WF_checked_term :
+Local Parameter WF_checked_term :
   forall Denv Sigma vars rels t dom, 
   check_term Denv Sigma vars rels t dom = true ->
   WF_term Denv Sigma vars rels t dom.
-Variable WF_checked_args :
+Local Parameter WF_checked_args :
   forall Denv Sigma vars rels args doms, 
   check_args Denv Sigma vars rels args doms = true ->
   WF_args Denv Sigma vars rels args doms.
 
-Variable WF_ground_term_term : 
+Local Parameter WF_ground_term_term : 
   forall Denv Sigma vars rels t dom,
   WF_ground_term Denv Sigma vars t dom ->
   WF_term Denv Sigma vars rels t dom.
 
-Variable WF_term_nil_ground_term :
+Local Parameter WF_term_nil_ground_term :
   forall Denv Sigma vars t dom,
   WF_term Denv Sigma vars nil t dom ->
   WF_ground_term Denv Sigma vars t dom.
 
-Variable interp_term: forall Denv,
+Local Parameter interp_term: forall Denv,
   signature Denv -> var_env Denv -> rel_env Denv -> term -> 
   forall (expected:domain), option (interp_domain Denv expected).
-Variable interp_args: forall Denv,
+Local Parameter interp_args: forall Denv,
   signature Denv -> var_env Denv -> rel_env Denv -> args -> 
   forall (doms:arity) (S:Type), abstract Denv doms S -> Poption S.
 
-Variable interp_WF_ground_term_Some : 
+Local Parameter interp_WF_ground_term_Some : 
   forall Denv Sigma V F Venv,
   Instanceof Denv V F Venv->
   forall t dom, 
   WF_ground_term Denv Sigma V t dom ->
   (exists x, interp_term Denv Sigma Venv nil t dom = Some x).
 
-Variable term_eq_refl: forall Denv Sigma vars rels dom t1 t2,
+Local Parameter term_eq_refl: forall Denv Sigma vars rels dom t1 t2,
   term_eq t1 t2 = true -> 
   interp_term Denv Sigma vars rels t1 dom =  
   interp_term Denv Sigma vars rels t2 dom.
-Variable args_eq_refl: forall Denv Sigma vars rels doms T hd a1 a2,
+Local Parameter args_eq_refl: forall Denv Sigma vars rels doms T hd a1 a2,
   args_eq a1 a2 = true -> 
   interp_args Denv Sigma vars rels a1 doms T hd =  
   interp_args Denv Sigma vars rels a2 doms T hd.
 
-Variable WF_term_instx : forall Denv Sigma V (F:Full V) rels dom t expected,
+Local Parameter WF_term_instx : forall Denv Sigma V (F:Full V) rels dom t expected,
 WF_term Denv Sigma V (rels ++ dom :: nil) t expected ->
 WF_term Denv Sigma (V \ dom) rels
   (inst_term (mkVar (index V)) (length rels) t) expected.
-Variable WF_args_instx : forall Denv Sigma V (F:Full V) rels dom a doms,
+Local Parameter WF_args_instx : forall Denv Sigma V (F:Full V) rels dom a doms,
 WF_args Denv Sigma V (rels ++ dom :: nil) a doms ->
 WF_args Denv Sigma (V \ dom) rels
   (inst_args (mkVar (index V)) (length rels) a) doms.
 
-Variable term_instx : forall Denv Sigma V F Venv, Instanceof Denv V F Venv ->
+Local Parameter term_instx : forall Denv Sigma V F Venv, Instanceof Denv V F Venv ->
 forall dom rel rels t expected, WF_term Denv Sigma V 
 (List.map (E_domain Denv) (rels ++ (mkE Denv dom rel) :: nil)) t expected ->
 interp_term Denv Sigma (Venv\mkE Denv dom rel) rels
     (inst_term (mkVar (index V)) (length rels) t) expected =
 interp_term Denv Sigma Venv (rels ++ (mkE Denv dom rel) :: nil) t expected.
 
-Variable args_instx : forall Denv Sigma V F Venv, Instanceof Denv V F Venv ->
+Local Parameter args_instx : forall Denv Sigma V F Venv, Instanceof Denv V F Venv ->
 forall dom rel rels a doms (T:Type) head, WF_args Denv Sigma V 
 (List.map (E_domain Denv) (rels ++ (mkE Denv dom rel) :: nil)) a doms ->
 interp_args Denv Sigma (Venv\mkE Denv dom rel) rels
@@ -106,19 +106,19 @@ interp_args Denv Sigma (Venv\mkE Denv dom rel) rels
 interp_args Denv Sigma Venv (rels ++ (mkE Denv dom rel) :: nil) a doms T
      head.
 
-Variable WF_term_inst : forall Denv Sigma V t dom,
+Local Parameter WF_term_inst : forall Denv Sigma V t dom,
 WF_ground_term Denv Sigma V t dom ->
 forall rels tt dd,
 WF_term Denv Sigma V (rels ++ dom :: nil) tt dd ->
 WF_term Denv Sigma V rels (inst_term t (length rels) tt) dd.
 
-Variable WF_args_inst : forall Denv Sigma V t dom,
+Local Parameter WF_args_inst : forall Denv Sigma V t dom,
 WF_ground_term Denv Sigma V t dom ->
 forall rels a doms,
 WF_args Denv Sigma V (rels ++ dom :: nil) a doms ->
 WF_args Denv Sigma V rels (inst_args t (length rels) a) doms.
 
-Variable term_inst : forall Denv Sigma V F Venv t dom x, 
+Local Parameter term_inst : forall Denv Sigma V F Venv t dom x, 
 Instanceof Denv V F Venv -> 
 WF_ground_term Denv Sigma V t dom ->
 interp_term Denv Sigma Venv nil t dom = Some x ->
@@ -128,7 +128,7 @@ WF_term Denv Sigma V
 interp_term Denv Sigma Venv (rels ++ (mkE Denv dom x) :: nil) tt dd =
 interp_term Denv Sigma Venv rels (inst_term t (length rels) tt) dd.
 
-Variable args_inst : forall Denv Sigma V F Venv t dom x,
+Local Parameter args_inst : forall Denv Sigma V F Venv t dom x,
 Instanceof Denv V F Venv -> 
 WF_ground_term Denv Sigma V t dom ->
 interp_term Denv Sigma Venv nil t dom = Some x ->
@@ -138,45 +138,45 @@ WF_args Denv Sigma V
 interp_args Denv Sigma Venv (rels ++ (mkE Denv dom x) :: nil) a doms T P =
 interp_args Denv Sigma Venv rels (inst_args t (length rels) a) doms T P.
 
-Variable Weak_WF_term : forall Denv Sigma vars dom rels t expected,
+Local Parameter Weak_WF_term : forall Denv Sigma vars dom rels t expected,
 Full vars ->
 WF_term Denv Sigma vars rels t expected ->
 WF_term Denv Sigma (vars\dom) rels t expected.
-Variable Weak_WF_args : forall Denv Sigma vars dom rels a doms,
+Local Parameter Weak_WF_args : forall Denv Sigma vars dom rels a doms,
 Full vars ->
 WF_args Denv Sigma vars rels a doms ->
 WF_args Denv Sigma (vars\dom) rels a doms.
 
-Variable Weak_interp_term: forall Denv Sigma V F Venv var t rels expected,
+Local Parameter Weak_interp_term: forall Denv Sigma V F Venv var t rels expected,
 Instanceof Denv V F Venv ->
 WF_term Denv Sigma V (List.map (E_domain Denv) rels) t expected ->
 interp_term Denv Sigma Venv rels t expected=
 interp_term Denv Sigma (Venv\var)  rels t expected.
-Variable Weak_interp_args: forall Denv Sigma V F Venv var S rels a doms Kont,
+Local Parameter Weak_interp_args: forall Denv Sigma V F Venv var S rels a doms Kont,
 Instanceof Denv V F Venv ->
 WF_args Denv Sigma V (List.map (E_domain Denv) rels) a doms ->
 interp_args Denv Sigma Venv rels a doms S Kont=
 interp_args Denv Sigma (Venv\var) rels a doms S Kont.
 
-Variable Bind_WF_term: forall Denv Sigma vars delta rels t expected,
+Local Parameter Bind_WF_term: forall Denv Sigma vars delta rels t expected,
 WF_term Denv Sigma vars rels t expected ->
 WF_term Denv Sigma vars (rels ++ delta) t expected.
-Variable Bind_WF_args : forall Denv Sigma vars delta rels a doms,
+Local Parameter Bind_WF_args : forall Denv Sigma vars delta rels a doms,
 WF_args Denv Sigma vars rels a doms ->
 WF_args Denv Sigma vars (rels ++ delta) a doms.
 
-Variable Bind_interp_term: forall Denv Sigma V F Venv delta rels t expected,
+Local Parameter Bind_interp_term: forall Denv Sigma V F Venv delta rels t expected,
 Instanceof Denv V F Venv ->
 WF_term Denv Sigma V (List.map (E_domain Denv) rels) t expected ->
 interp_term Denv Sigma Venv rels t expected =
 interp_term Denv Sigma Venv (rels++delta) t expected.
-Variable Bind_interp_args: forall Denv Sigma V F Venv delta S rels a doms Kont,
+Local Parameter Bind_interp_args: forall Denv Sigma V F Venv delta S rels a doms Kont,
 Instanceof Denv V F Venv ->
 WF_args Denv Sigma V (List.map (E_domain Denv) rels) a doms ->
 interp_args Denv Sigma Venv rels a doms S Kont=
 interp_args Denv Sigma Venv (rels++delta) a doms S Kont.
 
-Variable WF_rewrite_term : forall Denv Sigma vars dom t1 t2 rels,
+Local Parameter WF_rewrite_term : forall Denv Sigma vars dom t1 t2 rels,
 WF_ground_term Denv Sigma vars t1 dom ->
 WF_ground_term Denv Sigma vars t2 dom ->
 forall t occ rt expected,
@@ -184,7 +184,7 @@ rewrite_term t1 t2 occ t = Some rt ->
 WF_term Denv Sigma vars rels t expected ->
 WF_term Denv Sigma vars rels rt expected.
 
-Variable WF_rewrite_args : forall Denv Sigma vars dom t1 t2 rels,
+Local Parameter WF_rewrite_args : forall Denv Sigma vars dom t1 t2 rels,
 WF_ground_term Denv Sigma vars t1 dom ->
 WF_ground_term Denv Sigma vars t2 dom ->
 forall a occ ra doms,
@@ -192,7 +192,7 @@ rewrite_args t1 t2 occ a = Some ra ->
 WF_args Denv Sigma vars rels a doms ->
 WF_args Denv Sigma vars rels ra doms.
 
-Variable term_rewrite : forall Denv Sigma V F Venv,
+Local Parameter term_rewrite : forall Denv Sigma V F Venv,
 Instanceof Denv V F Venv->
 forall dom t1 t2 it1 it2,  
 WF_ground_term Denv Sigma V t1 dom ->
@@ -206,7 +206,7 @@ WF_term Denv Sigma V (List.map (E_domain Denv) rels) t expected ->
 interp_term Denv Sigma Venv rels t expected =
 interp_term Denv Sigma Venv rels rt expected.
 
-Variable args_rewrite :
+Local Parameter args_rewrite :
 forall Denv Sigma V F Venv,
 Instanceof Denv V F Venv->
 forall dom t1 t2 it1 it2,  
